cava/monad-examples/Sorter.v
@@ -1,0 +1,123 @@
+(****************************************************************************)
+(* Copyright 2020 The Project Oak Authors                                   *)
+(*                                                                          *)
+(* Licensed under the Apache License, Version 2.0 (the "License")           *)
+(* you may not use this file except in compliance with the License.         *)
+(* You may obtain a copy of the License at                                  *)
+(*                                                                          *)
+(*     http://www.apache.org/licenses/LICENSE-2.0                           *)
+(*                                                                          *)
+(* Unless required by applicable law or agreed to in writing, software      *)
+(* distributed under the License is distributed on an "AS IS" BASIS,        *)
+(* WITHOUT WARRANTIES OR CONDITIONS OF ANY KIND, either express or implied. *)
+(* See the License for the specific language governing permissions and      *)
+(* limitations under the License.                                           *)
+(****************************************************************************)
+
+Require Import ExtLib.Structures.Monads.
+
+From Coq Require Import Ascii String.
+
+From Coq Require Import Lists.List.
+Import ListNotations.
+
+From Coq Require Import Vector.
+From Coq Require Import Bool.Bvector.
+Import VectorNotations.
+
+From Coq Require Import NArith.Ndigits.
+
+Require Import Cava.Cava.
+Require Import Cava.VectorUtils.
+Require Import Cava.Monad.CavaMonad.
+
+From Coq Require Import Lia Omega.
+
+Local Open Scope vector_scope.
+
+Definition twoSorter {m bit} `{Cava m bit} {n}
+                     (ab: smashTy bit (BitVec (BitVec Bit n) 2)) :
+                     m (Vector.t (Vector.t bit n) 2) :=
+   let a := @Vector.nth_order _ 2 ab 0 (ltac:(lia)) in
+   let b := @Vector.nth_order _ 2 ab 1 (ltac:(lia)) in
+   comparison <- greaterThanOrEqual a b ;;
+   negComparison <- inv comparison ;;
+   let sorted : Vector.t (Vector.t bit n) 2 := [indexAt ab [comparison];
+                                                indexAt ab [negComparison]] in
+   ret sorted.
+
+Definition two_sorter_Interface bitSize
+  := combinationalInterface "two_sorter"
+     (mkPort "inputs" (BitVec (BitVec Bit bitSize) 2))
+     (mkPort "sorted" (BitVec (BitVec Bit bitSize) 2))
+     [].
+
+Definition two_sorter_Netlist
+  := makeNetlist (two_sorter_Interface 8) twoSorter.
+
+Definition v0 := N2Bv_sized 8   5.
+Definition v1 := N2Bv_sized 8 157.
+Definition v2 := N2Bv_sized 8 255.
+Definition v3 := N2Bv_sized 8  63.
+
+Definition two_sorter_tb_inputs : list (Vector.t (Bvector 8) _) :=
+  [[v0; v1];
+   [v1; v0];
+   [v1; v2];
+   [v2; v1];
+   [v2; v3];
+   [v3; v2]
+  ].
+
+Definition adder_tree4_8_tb_expected_outputs : list (Vector.t (Bvector 8) _) :=
+  map (fun i => combinational (twoSorter i)) two_sorter_tb_inputs.
+
+Definition two_sorter_tb :=
+  testBench "two_sorter_tb" (two_sorter_Interface 8)
+  two_sorter_tb_inputs adder_tree4_8_tb_expected_outputs.
+
+Definition twoSorterSpec {bw: nat} (ab : Vector.t (Bvector bw) 2) :
+                                   Vector.t (Bvector bw) 2 :=
+  let a := @Vector.nth_order _ 2 ab 0 (ltac:(lia)) in
+  let b := @Vector.nth_order _ 2 ab 1 (ltac:(lia)) in
+  if N.to_nat (Bv2N b) <=? N.to_nat (Bv2N a) then
+    [b; a]
+  else
+    [a; b].                                      
+
+Lemma two_sorter_correct: forall (n m: nat) (a b: Bvector m),
+      combinational (twoSorter [a; b]) = twoSorterSpec [a; b].
+Proof.
+Abort. (* Proof unfolds in a complicated way. *)
+
+(*
+
+TODO: Fix type error:
+Error:
+In environment
+unpair : forall n : nat, t (nat * nat) n -> t nat (2 * n)
+n : nat
+v : t (nat * nat) n
+n' : nat
+v0 : t (nat * nat) (S n')
+x : nat * nat
+xs : t (nat * nat) n'
+a : nat
+b : nat
+The term "a :: b :: unpair n' xs" has type "t nat (S (S (2 * n')))"
+while it is expected to have type "t nat (2 * S n')".
+
+Fixpoint unpair {n} (v: Vector.t (nat * nat) n) : Vector.t nat (2*n) :=
+  match n, v return Vector.t nat (2*n) with
+  | O, vv => []
+  | S n', vv => let (x, xs) := Vector.uncons v in
+                let (a, b) := x in
+                a :: b :: unpair xs
+  end.
+
+Definition riffle {n} (v: Vector.t nat (2*n)) : Vector.t nat (2*n) :=
+  let '(a, b) := halveV v in
+  let abz := vcombine a b in
+  unpair abz.
+
+*)
